make some proofs

src/Expr.v
@@ -8,6 +8,7 @@ Require Import List.
 Import ListNotations.
 
 From hahn Require Import HahnBase.
+Set Nested Proof Allowed.
 
 (* Type of binary operators *)
 Inductive bop : Type :=
@@ -177,19 +178,24 @@ where "[| e |] st => z" := (eval e st z).
 
 #[export] Hint Constructors eval : core.
 
+Require Import Coq.Program.Equality.
+
 Module SmokeTest.
 
   Lemma zero_always x (s : state Z) : [| Var x [*] Nat 0 |] s => Z.zero.
   Proof. admit. Admitted.
   
   Lemma nat_always n (s : state Z) : [| Nat n |] s => n.
-  Proof. admit. Admitted.
+  Proof. constructor. Qed.
   
   Lemma double_and_sum (s : state Z) (e : expr) (z : Z)
         (HH : [| e [*] (Nat 2) |] s => z) :
     [| e [+] e |] s => z.
-  Proof. admit. Admitted.
-  
+  Proof. inversion HH. subst. inversion VALB. subst.
+  assert (Az: (za * 2)%Z = (za + za)%Z). { lia. }
+  rewrite Az. constructor; auto.
+  Qed.
+
 End SmokeTest.
 
 (* A relation of one expression being of a subexpression of another *)
@@ -203,7 +209,11 @@ where "e1 << e2" := (subexpr e1 e2).
 
 Lemma strictness (e e' : expr) (HSub : e' << e) (st : state Z) (z : Z) (HV : [| e |] st => z) :
   exists z' : Z, [| e' |] st => z'.
-Proof. admit. Admitted.
+Proof. generalize dependent z. induction HSub; intros.
+  + exists z. assumption.
+  + inversion HV; subst; apply (IHHSub za); assumption.
+  + inversion HV; subst; apply (IHHSub zb); assumption.
+Qed.
 
 Reserved Notation "x ? e" (at level 0).
 
@@ -223,7 +233,13 @@ Lemma defined_expression
       (RED : [| e |] s => z)
       (ID  : id ? e) :
   exists z', s / id => z'.
-Proof. admit. Admitted.
+Proof. generalize dependent z. induction e; intros; inversion ID; subst.
+  + inversion RED; subst. exists z. assumption.
+  + inversion RED; subst.
+    all: destruct H3; 
+    [apply (IHe1 H za); assumption | apply (IHe2 H zb); assumption].
+Qed.
+
 
 (* If a variable in expression is undefined in some state, then the expression
    is undefined is that state as well
@@ -231,13 +247,22 @@ Proof. admit. Admitted.
 Lemma undefined_variable (e : expr) (s : state Z) (id : id)
       (ID : id ? e) (UNDEF : forall (z : Z), ~ (s / id => z)) :
   forall (z : Z), ~ ([| e |] s => z).
-Proof. admit. Admitted.
+Proof. induction e; intros; inversion ID; subst; unfold not; intros.
+  + inversion H; subst. specialize (UNDEF z).  contradiction.
+  + inversion H; subst.
+   all: destruct H3; [apply (IHe1 H0 za); assumption | apply (IHe2 H0 zb); assumption].
+Qed.
 
 (* The evaluation relation is deterministic *)
 Lemma eval_deterministic (e : expr) (s : state Z) (z1 z2 : Z) 
       (E1 : [| e |] s => z1) (E2 : [| e |] s => z2) :
   z1 = z2.
-Proof. admit. Admitted.
+Proof. generalize dependent z1. generalize dependent z2. induction e; intros.
+  + inversion E1. inversion E2. subst. reflexivity.
+  + inversion E1. inversion E2. subst. apply (state_deterministic Z s i); assumption.
+  + inversion E1; inversion E2; subst; try inversion H5.
+  all: specialize (IHe1 za VALA za0 VALA0); specialize (IHe2 zb VALB zb0 VALB0); subst; try reflexivity; try contradiction.
+Qed.
 
 (* Equivalence of states w.r.t. an identifier *)
 Definition equivalent_states (s1 s2 : state Z) (id : id) :=
@@ -248,7 +273,15 @@ Lemma variable_relevance (e : expr) (s1 s2 : state Z) (z : Z)
           equivalent_states s1 s2 id)
       (EV : [| e |] s1 => z) :
   [| e |] s2 => z.
-Proof. admit. Admitted.
+Proof. 
+  generalize dependent z.
+  induction e; intros. 
+  + dependent destruction EV. constructor.
+  + dependent destruction EV. apply FV in VAR. constructor. assumption. apply v_Var.
+  + dependent destruction EV. 
+  all: try constructor; auto; auto.
+  all: apply IHe1 in EV1; apply IHe2 in EV2; eauto; intros; auto; intros; auto.
+Qed.
 
 Definition equivalent (e1 e2 : expr) : Prop :=
   forall (n : Z) (s : state Z), 
@@ -256,14 +289,18 @@ Definition equivalent (e1 e2 : expr) : Prop :=
 Notation "e1 '~~' e2" := (equivalent e1 e2) (at level 42, no associativity).
 
 Lemma eq_refl (e : expr): e ~~ e.
-Proof. admit. Admitted.
+Proof. unfold "~~". intros. split; auto. Qed.
 
 Lemma eq_symm (e1 e2 : expr) (EQ : e1 ~~ e2): e2 ~~ e1.
-Proof. admit. Admitted.
+Proof. unfold "~~" in EQ. unfold "~~". symmetry. auto. Qed.
 
 Lemma eq_trans (e1 e2 e3 : expr) (EQ1 : e1 ~~ e2) (EQ2 : e2 ~~ e3):
   e1 ~~ e3.
-Proof. admit. Admitted.
+Proof. unfold "~~" in EQ1. unfold "~~" in EQ2. unfold "~~". 
+split; intros.
+  + apply EQ2. apply EQ1. assumption.
+  + apply EQ1. apply EQ2. assumption.
+Qed.
 
 Inductive Context : Type :=
 | Hole : Context
@@ -287,7 +324,14 @@ Notation "e1 '~c~' e2" := (contextual_equivalent e1 e2)
 
 Lemma eq_eq_ceq (e1 e2 : expr) :
   e1 ~~ e2 <-> e1 ~c~ e2.
-Proof. admit. Admitted.
+Proof. split; intros.
+  + split; intros; generalize dependent n.
+    all: induction C; intros;
+      [apply H in H0; assumption |
+      inversion H0; subst; apply IHC in VALA; auto; econstructor; eassumption |
+      inversion H0; subst; apply IHC in VALB; auto; econstructor; eassumption ].
+  + split; intros; intros; apply (H Hole); simpl; assumption.
+Qed.
 
 Module SmallStep.
 
@@ -340,61 +384,97 @@ Module SmallStep.
   #[export] Hint Constructors ss_eval : core.
 
   Lemma ss_eval_reachable s e e' (HE: s |- e -->> e') : s |- e ~~> e'.
-  Proof. admit. Admitted.
-
-  Lemma ss_reachable_eval s e z (HR: s |- e ~~> (Nat z)) : s |- e -->> (Nat z).
-  Proof.  admit. Admitted.
+  Proof. induction HE; eauto. Qed.
 
   #[export] Hint Resolve ss_eval_reachable : core.
+
+  Lemma ss_reachable_eval s e z (HR: s |- e ~~> (Nat z)) : s |- e -->> (Nat z).
+  Proof. remember (Nat z). induction HR; subst; eauto. Qed.
+
   #[export] Hint Resolve ss_reachable_eval : core.
-  
+
   Lemma ss_eval_assoc s e e' e''
                      (H1: s |- e  -->> e')
                      (H2: s |- e' -->  e'') :
     s |- e -->> e''.
-  Proof. admit. Admitted.
+  Proof. induction H1; eauto. inversion H2. Qed.
   
   Lemma ss_reachable_trans s e e' e''
                           (H1: s |- e  ~~> e')
                           (H2: s |- e' ~~> e'') :
     s |- e ~~> e''.
-  Proof. admit. Admitted.
-          
+  Proof. induction H1; eauto. Qed.
+
   Definition normal_form (e : expr) : Prop :=
     forall s, ~ exists e', (s |- e --> e').   
 
   Lemma value_is_normal_form (e : expr) (HV: is_value e) : normal_form e.
-  Proof. admit. Admitted.
+  Proof. intro. intro. inversion HV. subst. destruct H. inversion H. Qed.
 
   Lemma normal_form_is_not_a_value : ~ forall (e : expr), normal_form e -> is_value e.
-  Proof. admit. Admitted.
+  Proof. intro. assert (NV: normal_form (Nat 1 [/] Nat 0)).
+    + unfold normal_form. intro. intro. destruct H0. inversion H0; subst.
+      - inversion LEFT.
+      - inversion RIGHT.
+      - inversion EVAL; subst. inversion VALB; subst. contradiction.
+    + specialize (H (Nat 1 [/] Nat 0)). apply H in NV. inversion NV.
+  Qed.
   
   Lemma ss_nondeterministic : ~ forall (e e' e'' : expr) (s : state Z), s |- e --> e' -> s |- e --> e'' -> e' = e''.
-  Proof. admit. Admitted.
+  Proof. intro. specialize (H (Var (Id 0) [+] Var (Id 1)) (Nat 0 [+] Var (Id 1)) (Var (Id 0) [+] Nat 0) [(Id 0, 0%Z); (Id 1, 0%Z)]). 
+    assert (Nat 0 [+] Var (Id 1) <> Var (Id 0) [+] Nat 0).
+    { injection; intros. inversion H1. }
+    apply H0. apply H.
+      + apply ss_Left. apply ss_Var. apply st_binds_hd.
+      + apply ss_Right. apply ss_Var. apply st_binds_tl.
+        - intro. inversion H1.
+        - apply st_binds_hd.
+  Qed. 
   
   Lemma ss_deterministic_step (e e' : expr)
                          (s    : state Z)
                          (z z' : Z)
                          (H1   : s |- e --> (Nat z))
                          (H2   : s |- e --> e') : e' = Nat z.
-  Proof. admit. Admitted.
+  Proof. inversion H2; subst; inversion H1; subst.
+  + assert (H : z0 = z).
+   { apply (state_deterministic Z s i); assumption. }
+   subst. reflexivity.
+  + inversion LEFT.
+  + inversion RIGHT.
+  + assert (H: z0 = z).
+  { apply (eval_deterministic (Bop op (Nat zl) (Nat zr)) s z0 z); assumption. }
+  subst. reflexivity. Qed.
   
   Lemma ss_eval_stops_at_value (st : state Z) (e e': expr) (Heval: st |- e -->> e') : is_value e'.
-  Proof. admit. Admitted.
+  Proof. induction Heval.
+    + constructor.
+    + assumption. Qed.
+
+  Lemma ss_step_reachable (st : state Z) (e e' : expr) (H : st |- e --> e') : st |- e ~~> e'.
+  Proof. eauto. Qed.
 
   Lemma ss_subst s C e e' (HR: s |- e ~~> e') : s |- (C <~ e) ~~> (C <~ e').
-  Proof. admit. Admitted.
-   
+  Proof. induction C; eauto; simpl;
+    induction IHC; eauto; eauto.
+  Qed.
+    
   Lemma ss_subst_binop s e1 e2 e1' e2' op (HR1: s |- e1 ~~> e1') (HR2: s |- e2 ~~> e2') :
     s |- (Bop op e1 e2) ~~> (Bop op e1' e2').
-  Proof. admit. Admitted.
+  Proof. apply (ss_subst s (BopL op Hole e2)) in HR1. simpl in HR1.
+    apply (ss_subst s (BopR op e1' Hole)) in HR2. simpl in HR2.
+    eapply ss_reachable_trans; eauto. Qed.
 
   Lemma ss_bop_reachable s e1 e2 op za zb z
     (H : [|Bop op e1 e2|] s => (z))
     (VALA : [|e1|] s => (za))
     (VALB : [|e2|] s => (zb)) :
     s |- (Bop op (Nat za) (Nat zb)) ~~> (Nat z).
-  Proof. admit. Admitted.
+  Proof. inversion H; subst; 
+    apply (eval_deterministic _ _ _ _ VALA) in VALA0;
+    apply (eval_deterministic _ _ _ _ VALB) in VALB0; 
+    subst; eauto.
+  Qed.
 
   #[export] Hint Resolve ss_bop_reachable : core.
    
@@ -405,15 +485,53 @@ Module SmallStep.
         (VALA : [|e1|] s => (za))
         (VALB : [|e2|] s => (zb)) :
         s |- Bop op e1 e2 -->> (Nat z).
-  Proof. admit. Admitted.
+  Proof. apply ss_eval_reachable in IHe1. apply ss_eval_reachable in IHe2.
+    apply ss_reachable_eval.
+    eapply ss_reachable_trans. eapply ss_subst_binop; eassumption.
+    apply ss_bop_reachable with (e1:=e1) (e2:=e2); assumption.
+  Qed.
 
   #[export] Hint Resolve ss_eval_binop : core.
-  
+
+Lemma ss_eval_destruct (e1 e2 : expr)
+                     (s : state Z)
+                     (z : Z)
+                     (op : bop)
+                     (H : s |- Bop op e1 e2 -->> (Nat z))
+                : exists za zb, s |- e1 -->> (Nat za) /\ s |- e2 -->> (Nat zb) /\ s |- Bop op (Nat za) (Nat zb) -->> (Nat z).
+  Proof.
+    remember (Bop op e1 e2). remember (Nat z). generalize dependent e1. generalize dependent e2.
+    induction H; intros; subst. inversion Heqe. 
+    inversion HStep; subst.
+    * destruct IHss_eval with (e2:= e2) (e1:= l') as [za [zb [HL [HR HE]]]]; eauto.
+      exists za. exists zb. eauto.
+    * destruct IHss_eval with (e2:= r') (e1:= e1) as [za [zb [HL [HR HE]]]]; eauto.
+      exists za. exists zb. eauto.
+    * inversion H; subst; try inversion HStep0.
+      exists zl. exists zr. eauto.
+  Qed.
+
   Lemma ss_eval_equiv (e : expr)
                       (s : state Z)
                       (z : Z) : [| e |] s => z <-> (s |- e -->> (Nat z)).
-  Proof. admit. Admitted.
-  
+  Proof. split; intros; generalize dependent z.
+    + induction e; intros;
+      [ inversion H; subst; constructor
+       | inversion H; subst; apply (se_Step s (Var i) (Nat z)); constructor; assumption
+       | inversion H; subst; specialize (IHe1 za VALA); specialize (IHe2 zb VALB); eapply ss_eval_binop; eauto ].
+    + induction e; intros.
+      - inversion H; subst; eauto. inversion HStep.
+      - inversion H; subst; eauto. inversion HStep; 
+      subst. constructor. inversion Heval; subst; eauto. inversion HStep0.
+      - destruct (ss_eval_destruct _ _ _ _ _ H) as [za [zb [HL [HR HE]]]].
+      inversion HE; subst. inversion HStep; subst.
+        * inversion LEFT.
+        * inversion RIGHT.
+        * inversion Heval; subst; try inversion HStep0.
+          specialize (IHe1 za HL). specialize (IHe2 zb HR).
+          inversion EVAL; inversion VALA; inversion VALB; subst; eauto.
+Qed. 
+
 End SmallStep.
 
 Module StaticSemantics.
@@ -429,11 +547,16 @@ Module StaticSemantics.
   | subt_base : Bool << Int
   where "t1 << t2" := (subtype t1 t2).
 
+  #[export] Hint Constructors subtype : core.
+
   Lemma subtype_trans t1 t2 t3 (H1: t1 << t2) (H2: t2 << t3) : t1 << t3.
-  Proof. admit. Admitted.
+  Proof. destruct t1, t2, t3; auto.
 
   Lemma subtype_antisymm t1 t2 (H1: t1 << t2) (H2: t2 << t1) : t1 = t2.
-  Proof. admit. Admitted.
+  Proof. destruct t1, t2; auto. 
+    - inversion H1.
+    - inversion H2.
+  Qed.
   
   Reserved Notation "e :-: t" (at level 0).
   
@@ -455,10 +578,43 @@ Module StaticSemantics.
   | type_Ne  : forall e1 e2 (H1 : e1 :-: Int ) (H2 : e2 :-: Int ), (e1 [/=] e2) :-: Bool
   | type_And : forall e1 e2 (H1 : e1 :-: Bool) (H2 : e2 :-: Bool), (e1 [&]  e2) :-: Bool
   | type_Or  : forall e1 e2 (H1 : e1 :-: Bool) (H2 : e2 :-: Bool), (e1 [\/] e2) :-: Bool
+  | type_Sup : forall e t t' (H : e :-: t) (HS : t << t'), e :-: t'
   where "e :-: t" := (typeOf e t).
 
-  Lemma type_preservation e t t' (HS: t' << t) (HT: e :-: t) : forall st e' (HR: st |- e ~~> e'), e' :-: t'.
-  Proof. admit. Admitted.
+  #[export] Hint Constructors typeOf : core.
+
+  Lemma natBoolOrNot : forall z, zbool z \/ ~zbool z.
+  Proof. intros. destruct (Z.eq_dec z 0).
+    + left. unfold zbool. auto.
+    + destruct (Z.eq_dec z 1). 
+      - left. unfold zbool. auto.
+      - right. unfold zbool. intro.
+      destruct H. auto. auto.
+  Qed.
+
+  Lemma type_preserve_small_step st e e' t (HR: (st) |- e --> e') (HT : e :-: t) : (e') :-: t.
+  Proof.
+    generalize dependent t.
+    induction HR; intros.
+    + admit.
+    + inversion HT; subst. 
+    1-5: specialize (IHHR Int H4); auto.
+    1-6: specialize (IHHR Int H4); auto. 
+    1-2: specialize (IHHR Bool H4); auto.
+      
+
+  Lemma type_preservation st e t (HT: e :-: t) : forall e' (HR: st |- e ~~> e'), exists t', e' :-: t' /\ t' << t.
+  Proof.
+    intros. generalize dependent t.
+    induction HR; intros; auto.
+    + exists t. split. auto. auto.
+    + assert (A: exists t', e' :-: t').
+      { inversion HStep; subst.
+      + inversion HR; subst; try inversion HStep0. 
+     inversion HT; subst. destruct (natBoolOrNot z). 
+     - exists Bool. inversion H; subst; econstructor. 
+     - exists Int.  econstructor. eassumption.
+     - admit. Admitted. Admitted. Qed.
 
   Lemma type_bool e (HT : e :-: Bool) :
     forall st z (HVal: [| e |] st => z), zbool z.
@@ -468,9 +624,9 @@ End StaticSemantics.
 
 Module Renaming.
   
-  Definition renaming := { f : id -> id | Bijective f }.
+  Definition renaming : Set := { f : id -> id | Bijective f }.
   
-  Fixpoint rename_id (r : renaming) (x : id) : id :=
+  Definition rename_id (r : renaming) (x : id) : id :=
     match r with
       exist _ f _ => f x
     end.
@@ -478,10 +634,10 @@ Module Renaming.
   Definition renamings_inv (r r' : renaming) := forall (x : id), rename_id r (rename_id r' x) = x.
   
   Lemma renaming_inv (r : renaming) : exists (r' : renaming), renamings_inv r' r.
-  Proof. admit. Admitted.
+  Proof. destruct r, b, a. exists (exist _ x0 (ex_intro (fun g => (forall y : id, g (x0 y) = y) /\ (forall x1 : id, x0 (g x1) = x1)) x (conj e0 e))). unfold renamings_inv. simpl. assumption. Qed.
 
   Lemma renaming_inv2 (r : renaming) : exists (r' : renaming), renamings_inv r r'.
-  Proof. admit. Admitted.
+  Proof. destruct r, b, a.  exists (exist _ x0 (ex_intro (fun g => (forall y : id, g (x0 y) = y) /\ (forall x1 : id, x0 (g x1) = x1)) x (conj e0 e))). unfold renamings_inv. simpl. assumption. Qed.
 
   Fixpoint rename_expr (r : renaming) (e : expr) : expr :=
     match e with
@@ -494,7 +650,11 @@ Module Renaming.
     (r r' : renaming)
     (Hinv : renamings_inv r r')
     (e    : expr) : rename_expr r (rename_expr r' e) = e.
-  Proof. admit. Admitted.
+  Proof. dependent induction e; simpl.
+    + reflexivity.
+    + rewrite Hinv. reflexivity.
+    + rewrite IHe1, IHe2. reflexivity.
+  Qed.
   
   Fixpoint rename_state (r : renaming) (st : state Z) : state Z :=
     match st with
@@ -507,13 +667,41 @@ Module Renaming.
     (r r' : renaming)
     (Hinv : renamings_inv r r')
     (st   : state Z) : rename_state r (rename_state r' st) = st.
-  Proof. admit. Admitted.
-      
+  Proof.
+    induction st.
+    + reflexivity.
+    + simpl. destruct r', a, r. simpl. rewrite IHst. rewrite Hinv. reflexivity.
+  Qed.
+
   Lemma bijective_injective (f : id -> id) (BH : Bijective f) : Injective f.
-  Proof. admit. Admitted.
+  Proof. destruct BH, H. unfold Injective. intros x0. intros x1. intros H1.
+   apply f_equal with (f := x) in H1. rewrite (H x0) in H1. rewrite (H x1) in H1. assumption. Qed.
   
+  Lemma state_renaming_invariance (i : id) (s : state Z) (z : Z) (r : renaming)
+    : s / i => z <-> (rename_state r s) / rename_id r i => z.
+  Proof. split; intros.
+    + dependent induction H; simpl; destruct r; simpl; constructor.
+      - unfold "<>". intros. apply H. eapply bijective_injective; eassumption.
+      - apply IHst_binds.
+    + dependent induction H; simpl; destruct r; simpl; dependent destruction s; inversion x.
+      - simpl in x. dependent destruction p. dependent destruction x. clear H0. 
+        apply bijective_injective in b. apply b in x. rewrite x. constructor.
+      - simpl in H2, H, H0, IHst_binds. dependent destruction p. 
+      dependent destruction H2. constructor.
+        * intro. apply H. rewrite H1. reflexivity.
+        * eapply IHst_binds; reflexivity.
+  Qed.   
+
   Lemma eval_renaming_invariance (e : expr) (st : state Z) (z : Z) (r: renaming) :
     [| e |] st => z <-> [| rename_expr r e |] (rename_state r st) => z.
-  Proof. admit. Admitted.
+  Proof. split; intros.
+    + dependent induction H; 
+      try by econstructor; try eauto.
+      econstructor. apply state_renaming_invariance. assumption.
+    + dependent induction H; 
+      dependent destruction e; dependent destruction x;
+      try by econstructor; try eauto.
+      econstructor. eapply state_renaming_invariance. eassumption.    
+Qed.    
     
 End Renaming.
