src/State.v
@@ -4,7 +4,8 @@ Require Import List.
 Import ListNotations.
 Require Import Lia.
 Require Export Arith Arith.EqNat.
-Require Export Id.
+Require Import Id.
+Require Import Coq.Program.Equality.
 
 Section S.
 
@@ -47,49 +48,90 @@ Section S.
     (SN : st / x => n)
     (SM : st / x => m) :
     n = m. 
-  Proof. admit. Admitted.
+  Proof.
+    induction st.
+    dependent destruction SN. dependent destruction SN.
+    + dependent destruction SM.
+      - reflexivity.
+      - contradiction.
+    + dependent destruction SM.
+      - contradiction.
+      - apply (IHst SN SM).  
+  Qed.
   
   Lemma update_eq (st : state) (x : id) (n : A) :
     st [x <- n] / x => n.
-  Proof. admit. Admitted.
+  Proof. unfold update. constructor. Qed.
 
   Lemma update_neq (st : state) (x2 x1 : id) (n m : A)
         (NEQ : x2 <> x1) : st / x1 => m <-> st [x2 <- n] / x1 => m.
-  Proof. admit. Admitted.
-  
+  Proof. split.
+  + intros H. apply neq_id_sym in NEQ. constructor; assumption.
+  + intros H. unfold update in H. dependent destruction H.
+    - contradiction.
+    - assumption.
+  Qed.
+
   Lemma update_shadow (st : state) (x1 x2 : id) (n1 n2 m : A) :
     st[x2 <- n1][x2 <- n2] / x1 => m <-> st[x2 <- n2] / x1 => m.
-  Proof. admit. Admitted.
+  Proof. split.
+    + intros H. dependent destruction H.
+      - unfold update. constructor.
+      - dependent destruction H0. contradiction. constructor; assumption.
+    + intros H. dependent destruction H.
+      - constructor.
+      - apply st_binds_tl.
+      { assumption. }
+      { apply st_binds_tl; assumption. }
+  Qed.
   
   Lemma update_same (st : state) (x1 x2 : id) (n1 m : A)
         (SN : st / x1 => n1)
         (SM : st / x2 => m) :
     st [x1 <- n1] / x2 => m.
-  Proof. admit. Admitted.
+  Proof.
+    destruct (id_eq_dec x1 x2).
+    + rewrite e. rewrite <- e in SM. apply (state_deterministic st x1 n1 m) in SN.
+      - rewrite SN. apply update_eq.
+      - assumption.
+    + apply st_binds_tl.
+      - apply neq_id_sym in n. assumption.
+      - assumption.
+  Qed.
   
   Lemma update_permute (st : state) (x1 x2 x3 : id) (n1 n2 m : A)
         (NEQ : x2 <> x1)
         (SM : st [x2 <- n1][x1 <- n2] / x3 => m) :
     st [x1 <- n2][x2 <- n1] / x3 => m.
-  Proof. admit. Admitted.
+  Proof.
+    apply neq_id_sym in NEQ. unfold update. unfold update in SM.
+    dependent destruction SM.
+    + apply st_binds_tl. assumption. constructor.
+    + dependent destruction SM.
+      - constructor.
+      - apply st_binds_tl. assumption. constructor; assumption.
+  Qed.
 
   Lemma state_extensional_equivalence (st st' : state) (H: forall x z, st / x => z <-> st' / x => z) : st = st'.
-  Proof. admit. Admitted.
+  Proof. Abort.
 
   Definition state_equivalence (st st' : state) := forall x a, st / x => a <-> st' / x => a.
 
   Notation "st1 ~~ st2" := (state_equivalence st1 st2) (at level 0).
 
   Lemma st_equiv_refl (st: state) : st ~~ st.
-  Proof. admit. Admitted.
+  Proof. unfold state_equivalence. tauto. Qed.
 
   Lemma st_equiv_symm (st st': state) (H: st ~~ st') : st' ~~ st.
-  Proof. admit. Admitted.
+  Proof. unfold state_equivalence. intros x a. split; intros; apply H; assumption. Qed.
 
   Lemma st_equiv_trans (st st' st'': state) (H1: st ~~ st') (H2: st' ~~ st'') : st ~~ st''.
-  Proof. admit. Admitted.
+  Proof. unfold state_equivalence. intros. split; intros.
+  + apply H2, H1. assumption.
+  + apply H1, H2. assumption.
+  Qed. 
 
   Lemma equal_states_equive (st st' : state) (HE: st = st') : st ~~ st'.
-  Proof. admit. Admitted.
-  
+  Proof. rewrite HE. apply st_equiv_refl. Qed.
+
 End S.
